# Problem Set 4

This problem set is self-assigned & does not appear in the lecture

2.4.14, 2.4.17, 2.4.19, 2.4.22, 2.4.23

---

(2.4.14) Let N be a normal subgroup of G and let $g \in G, n \in N$. Prove $g^{-1}ng \in N$

$N \triangleleft G$, so $\forall g \in G, gNg^{-1} = N$. This means that $g^{-1}Ng = N$ since $g^{-1} \in G$. In other words, conjugate $N$ by $g^{-1}$ instead of $g$.

(2.4.17) Prove that the center of a group is a normal subgroup

$\forall g \in G, gZ(G)g^{-1} = gg^{-1}Z(G) = Z(G)$, since $h \in Z(G) \implies hg = gh$

(2.4.19) Prove that if a group contains exactly one element of order 2, then that element is in the center of the group.

> **NOTE:** The below solution was obtained with help from [the corresponding question on *math.stackoverflow.com*](https://math.stackexchange.com/questions/821309/prove-that-if-a-group-contains-exactly-one-element-of-order-2-then-that-element). This question provided the "inspiration" to consider the element $z = y^{-1}gy$, and the rest was worked out on my own.

Let $g$ be the unique element of a group $G$ with order 2. Then consider the element $z = y^{-1}gy$, where $z, y \in G$. Then, $z^{2} = (y^{-1}gy)(y^{-1}gy) = y^{-1}g(yy^{-1})gy = y^{-1}(gg)y = y^{-1}y = e$. Since $g$ is the *unique* element of order two, this means that $z^{2} = g \implies gy = yg$

$
\newcommand{\map}[3]{
    #1 \colon #2 \rightarrow #3
}
$
(2.4.22) Let $\map{\phi}{G}{G'}$ be a surjective homomorphism.

(2.4.22a) Assume $G$ is cyclic. Prove that $G'$ is cyclic.

$\phi$ is surjective, so note that $Im\phi = G'$. Then, since every $h \in G$ can be written as $g^{k}$ for $k < o(g) = |G|, \phi(h) = \phi(g^{k}) = \phi(g)^{k}$, because $\phi$ is a homomorphism. Thus, every element $h' \in G'$ can be written as $\phi(g)^{k}$ (since $Im\phi = G'$), and therefore, $G'$ is cyclic, generated by $\phi(g)$.

(2.4.22b) Assume $G$ is abelian. Prove $G'$ is abelian.

$\phi$ is surjective, so every $g' \in G'$ can be written as $\phi(g)$ for some $g \in G$. Therefore, $g'h' = \phi(g)\phi(h) = \phi(gh) = \phi(hg) = \phi(h)\phi(g) = h'g'.$ Thus, $G'$ is abelian.

(2.4.23) Let $\map{\phi}{G}{G'}$ be a surjective homomorphism, and let $N \triangleleft G$. Prove $\phi(N) \triangleleft G'$.

> **NOTE:** The following proof received assistance from [the corresponding answer on *math.stackoverflow.com*](https://math.stackexchange.com/questions/219069/showing-that-if-a-subgroup-is-normal-its-surjective-homomorphic-image-is-norma). The answer in question helped clarify the definition of a normal subgroup -- I was originally thinking that $\phi(N)$ needed to be conjugated by elements of $G$, but the answer reminded me that $\phi(N)$ should be conjugated by elements of $G'$. All other work is my own.

Recall that $N \triangleleft G \implies gng^{-1} \in N, \forall g \in G$. In particular, if $\phi(N) \triangleleft G \implies g'\phi(n)g'^{-1} \in \phi(N), \forall g' \in G'$.

$\phi(N)$ is surjective, so every $g' \in G'$ can be written as $\phi(h)$ for some $h \in G$. Then, for $n \in N, g'\phi(n)g'^{-1} = \phi(h)\phi(n)\phi(h)^{-1} = \phi(hnh^{-1}) = \phi(m)$ where $m \in N$ (since $N \triangleleft G$). Therefore, $g'\phi(n)g'^{-1} \in \phi(N) \implies \phi(N) \triangleleft G'$